Hashmap/ForUpstream.lean
@@ -1,16 +1,26 @@
-
 /-
 Copyright (c) 2024 Lean FRO, LLC. All rights reserved.
 Released under Apache 2.0 license as described in the file LICENSE.
 Authors: Markus Himmel
 -/
-import Batteries.Data.List.Perm
 
 open List
 
 -- TODO
-theorem List.perm_append_comm_assoc (l₁ l₂ l₃ : List α) : l₁ ++ (l₂ ++ l₃) ~ l₂ ++ (l₁ ++ l₃) := by
-  simpa only [List.append_assoc] using perm_append_comm.append_right _
+
+theorem List.exists_of_set' {n : Nat} {a' : α} {l : List α} (h : n < l.length) :
+    ∃ l₁ l₂, l = l₁ ++ l.get ⟨n, h⟩ :: l₂ ∧ l₁.length = n ∧ l.set n a' = l₁ ++ a' :: l₂ := by
+  induction n generalizing a' l
+  · cases l
+    · simp at h
+    · next h t => refine ⟨[], t, by simp⟩
+  · next n ih =>
+    cases l
+    · simp at h; omega
+    · next a t =>
+      simp only [length_cons, Nat.succ_eq_add_one] at h
+      obtain ⟨t₁, t₂, ⟨ht₁, ht₂, ht₃⟩⟩ := ih (Nat.succ_lt_succ_iff.1 h)
+      exact ⟨a :: t₁, t₂, by simpa [ht₁, ht₂] using ht₁ ▸ ht₃⟩
 
 -- TODO: this is just about arrays
 theorem Array.exists_of_update (self : Array α) (i d h) :
@@ -54,18 +64,26 @@ theorem Nat.lt_of_eq_of_lt {n m k : Nat} : n = m → m < k → n < k :=
   fun h₁ h₂ => h₁ ▸ h₂
 
 -- From mathlib
-theorem List.Sublist.map (f : α → β) {l₁ l₂ : List α} (h : l₁.Sublist l₂) : (List.map f l₁).Sublist (List.map f l₂) := by
-  induction h
-  · simp
-  · exact Sublist.cons _ (by assumption)
-  · exact Sublist.cons₂ _ (by assumption)
-
--- From mathlib
 theorem List.isEmpty_iff {l : List α} : l.isEmpty ↔ l = [] := by
   cases l <;> simp
 
 theorem List.isEmpty_iff_length_eq_zero {l : List α} : l.isEmpty ↔ l.length = 0 := by
   rw [isEmpty_iff, length_eq_zero]
 
-theorem List.Perm.isEmpty_eq {l l' : List α} (h : l ~ l') : l.isEmpty = l'.isEmpty := by
-  cases l <;> cases l' <;> simp_all
+theorem List.get?_set_lt {n m : Nat} {l : List α} {a : α} (h : n < m) :
+    (l.set n a).get? m = l.get? m := by
+  induction l generalizing a n m
+  · simp
+  · next a t ih =>
+    obtain ⟨k, rfl⟩ := Nat.exists_eq_add_of_lt h
+    cases n
+    · simp
+    · simpa using ih (by omega)
+
+-- From batteries
+theorem List.drop_set_of_lt (a : α) {n m : Nat} (l : List α)
+    (hnm : n < m) : List.drop m (l.set n a) = List.drop m l := by
+  apply List.ext
+  intro k
+  simp only [get?_drop]
+  exact List.get?_set_lt (by omega)
